

Since cohomology is a homotopy invariant, we may substitute in the spaces above to this LES.

$$\begin{array}{ccccccc} \cdots & \longleftarrow & H^n(\mathbb{RP}^{n-1}) \oplus H^n(\mathbb{R}^n) & \longleftarrow & H^n(\mathbb{RP}^n) & \longleftarrow & \\ & & & & & & \uparrow \\ & & & & & & H^{n-1}(S^{n-1}) \longleftarrow H^{n-1}(\mathbb{RP}^{n-1}) \oplus H^{n-1}(\mathbb{R}^n) \longleftarrow H^{n-1}(\mathbb{RP}^n) \end{array}$$

Now we know the cohomology for spheres, and euclidean space, \mathbb{RP}^{n-1} is $n-1$ dimensional so that its n -th cohomology is zero and finally we already computed that $H^{n-1}(\mathbb{RP}^n) = 0$. Applying this we get

$$\begin{array}{ccccccc} \cdots & \longleftarrow & 0 & \longleftarrow & H^n(\mathbb{RP}^n) & \longleftarrow & \\ & & & & & & \uparrow \\ & & & & & & \mathbb{R} \longleftarrow H^{n-1}(\mathbb{RP}^{n-1}) \longleftarrow 0 \end{array}$$

Exactness of this sequence gives us that $\mathbb{R} \cong H^{n-1}(\mathbb{RP}^{n-1}) \oplus H^n(\mathbb{RP}^n)$ (the splitting is guaranteed since we were working with vector spaces). Now since $\mathbb{RP}^1 \cong S^1$, which has $H^1(S^1) \cong \mathbb{R}$, and the above formula holds for $n > 1$, we find recursively that for $n \geq 1$

$$H^n(\mathbb{RP}^n) \cong \begin{cases} \mathbb{R} & n \text{ odd} \\ 0 & n \text{ even} \end{cases}$$

From this and the fact that \mathbb{RP}^n is connected giving it 0-th cohomology \mathbb{R} , we get the cohomology ring

$$H^*(\mathbb{RP}^n) \cong \begin{cases} \mathbb{R}[x_n]/(x_n^2) & n \text{ odd} \\ \mathbb{R} & n \text{ even} \end{cases}$$

since the zero-th cohomology class is a unit with respect to wedge, and x_n represents the n -form $[\omega]$, but $\omega \wedge \omega = 0$ since $H^{2n}(\mathbb{RP}^n) = 0$ by dimension considerations. \square

2.

3. (a) The proof of the case $\alpha' = 0$ is identical to that of $\alpha = 0$, but we show that the rows rather than columns are linearly independent, so assume $v_1 \wedge \cdots \wedge v_p = \alpha \neq 0$. Now, it will suffice to show by induction that if $k < p$, then we can choose ω_{k+1} , so that

$$\left\{ \begin{pmatrix} \langle v_1, \omega_1 \rangle \\ \vdots \\ \langle v_p, \omega_1 \rangle \end{pmatrix}, \begin{pmatrix} \langle v_1, \omega_2 \rangle \\ \vdots \\ \langle v_p, \omega_2 \rangle \end{pmatrix}, \dots, \begin{pmatrix} \langle v_1, \omega_{k+1} \rangle \\ \vdots \\ \langle v_p, \omega_{k+1} \rangle \end{pmatrix} \right\} \subset \mathbb{R}^p$$

are linearly independent. Since $\alpha = v_1 \wedge \cdots \wedge v_p \neq 0$ we have necessarily that the v_j are linearly independent. Now since $k < p$, we can choose some $(x_1, \dots, x_p) \in \mathbb{R}^p$ linearly independent from the first k -columns, then $\omega = \omega_{k+1}$ can be constructed as follows, start with $\omega = \frac{x_1 v_1}{\|v_1\|^2}$ this is the base case, now assume recursively we have $\langle v_1, \omega \rangle = x_1, \dots, \langle v_j, \omega \rangle = x_j$, then we can take u to be the projection of v_{j+1} to $\text{span}\{v_1, \dots, v_j\}^\perp$, this is nonzero since $v_{j+1} \notin \text{span}\{v_1, \dots, v_j\}$. Then we have $\langle v_{j+1}, u \rangle = a \neq 0$ finally denote $\langle v_{j+1}, \omega \rangle = b$, and now take $\omega' = \omega + \frac{x_{j+1} - b}{a} u$, then since u is orthogonal to v_1, \dots, v_j , we still get $\langle v_i, \omega' \rangle = x_i$ for $i = 1, \dots, j$, but now we also get that

$$\langle v_{j+1}, \omega' \rangle = \langle v_{j+1}, \omega \rangle + \frac{x_{j+1} - b}{a} \langle v_{j+1}, u \rangle = b + \frac{x_{j+1} - b}{a} a = x_{j+1}$$

Continuing this process we get the desired ω_{k+1} , since this holds for any $k < p$, we can always construct some $\omega_1 \wedge \cdots \wedge \omega_p$ with the property that the columns of $(\langle v_i, \omega_j \rangle)_{1 \leq i, j \leq p}$ are linearly independent, and hence $\langle \alpha, \omega_1 \wedge \cdots \wedge \omega_p \rangle_p = \det(\langle v_i, \omega_j \rangle)_{1 \leq i, j \leq p} \neq 0$. \square

(b) Consider two positively oriented orthonormal bases e_1, \dots, e_k and d_1, \dots, d_k . Let T be the linear map defined by $T(e_i) = d_i$, and extending linearly, since both bases are positively oriented we get $\det T > 0$, moreover we have $(T^T T)_{ij} = \langle d_i, d_j \rangle = \delta_{ij}$, so that $T^T T = 1_V$ is orthogonal, since $\det T^T = \det T$, this relation gives us $(\det T)^2 = 1$, so $\det T = \pm 1$, but since we have established $\det T > 0$, we get to conclude that $\det T = 1$. Now we are done since

$$d_1 \wedge \dots \wedge d_k = T(e_1) \wedge \dots \wedge T(e_k) = (\det T)(e_1 \wedge \dots \wedge e_k) = e_1 \wedge \dots \wedge e_k$$

□

(c) We first consider an element of the form $\beta = e_{i_1} \wedge \dots \wedge e_{i_{k-p}}$ with $i_1 < i_2 < \dots < i_{k-p}$, now we can denote $\{j_1, \dots, j_p\} = \{1, \dots, k\} \setminus \{i_1, \dots, i_{k-p}\}$ with $j_1 < \dots < j_p$. It follows that $e_{j_1} \wedge \dots \wedge e_{j_p} \wedge \beta = (-1)^\ell \omega$ for some ℓ . I claim that $\star\beta = (-1)^\ell e_{j_1} \wedge \dots \wedge e_{j_p}$ satisfies $\lambda_\beta(\alpha) = \langle \alpha, \star\beta \rangle_p$. We first check this for α of the form $e_{r_1} \wedge \dots \wedge e_{r_p}$, since if it holds for elements of this form we get general elements of $\Lambda^p(V) = \sum a_i \alpha_i$ for a_i of this form, so that since λ_β is linear we get

$$\lambda_\beta(\sum a_i \alpha_i) = \sum a_i \lambda_\beta(\alpha_i) = \sum a_i \langle \alpha_i, \star\beta \rangle = \langle \sum a_i \alpha_i, \star\beta \rangle$$

so it suffices to check in this simplified case. Now if $\{r_1, \dots, r_p\} \cap \{i_1, \dots, i_{k-p}\} = \{i_z\} \neq \emptyset$, then we get $\alpha \wedge \beta = 0$, hence $\lambda_\beta(\alpha) = 0$, as well as the matrix with determinant $\langle \alpha, \star\beta \rangle_p$ having a row corresponding to $(\langle e_{i_z}, e_{j_1} \rangle, \dots, \langle e_{i_z}, e_{j_p} \rangle) = (0, \dots, 0)$, so that $\langle \alpha, \star\beta \rangle_p = 0$, now in the case that $\{r_1, \dots, r_p\} \cap \{i_1, \dots, i_{k-p}\} = \emptyset$, we get that $r_1, \dots, r_p = \sigma(j_1), \dots, \sigma(j_p)$ for $\sigma \in S_p$, then $e_{r_1} \wedge \dots \wedge e_{r_p} = \text{sgn}(\sigma) e_{j_1} \wedge \dots \wedge e_{j_p}$, so that $\alpha \wedge \beta = \text{sgn}(\sigma)(-1)^\ell \omega$, and $\langle \alpha \wedge \beta, \omega \rangle_k = \text{sgn}(\sigma)(-1)^\ell$, moreover $\langle \alpha, \star\beta \rangle = (-1)^\ell \det P_\sigma$ where P_σ denotes the permutation matrix taking $j_1 \mapsto \sigma(j_1)$, of course this is also equal to $(-1)^\ell \text{sgn}(\sigma)$, so we have provided existence of $\star\beta$ for β of the form $e_{i_1} \wedge \dots \wedge e_{i_{k-p}}$, from this we can establish existence for all β , since any $\beta \in \Lambda^{k-p}(V)$ can be written as $\sum a_i \beta_i$ for β_i of this form, this allows us to define $\star\beta = \sum a_i \star\beta_i$ then for any $\alpha \in \Lambda^p(V)$ we get

$$\begin{aligned} \lambda_\beta(\alpha) &= \langle \alpha \wedge \sum a_i \beta_i, \omega \rangle_k = \langle \sum a_i \alpha \wedge \beta_i, \omega \rangle_k = \sum a_i \langle \alpha \wedge \beta_i, \omega \rangle_k \\ &= \sum a_i \langle \alpha, \star\beta_i \rangle_p = \langle \alpha, \sum a_i \star\beta_i \rangle_p = \langle \alpha, \star\beta \rangle_p \end{aligned}$$

Which suffices to prove existence for any $\beta \in \Lambda^{k-p}(V)$. Now we need to check uniqueness. Suppose $\star\beta' = \star\beta$, then $\alpha \mapsto \langle \alpha \wedge (\beta - \beta'), \omega \rangle_k = 0$ for all α . Suppose now that $\beta \neq \beta'$, we can write $\beta = \sum a_i \beta_i$, and $\beta' = \sum b_i \beta'_i$ where β_i, β'_i are of the form $e_{i_1} \wedge \dots \wedge e_{i_{k-p}}$ for $i_1 < \dots < k-p$, it follows that the multiplicity of one of these summands must differ between β and β' , otherwise the two will be equal. So assume without loss of generality that $\beta_1 = \beta'_1$, but $a_1 \neq b_1$, moreover since one of them must be nonzero we can assume $a_1 \neq 0$. Now denote $\beta_1 = e_{i_1} \wedge \dots \wedge e_{i_{k-p}}$, and once again define $\{j_1, \dots, j_p\} = \{1, \dots, k\} \setminus \{i_1, \dots, i_{k-p}\}$ with $j_1 < \dots < j_p$, it follows that for $\alpha = e_{j_1} \wedge \dots \wedge e_{j_p}$ we have $\alpha \wedge \beta_\ell = 0$ for any $\ell \neq 1$, and same for β'_ℓ , since some j_z must appear in the wedge terms of β_ℓ (or respectively β'_ℓ) by virtue of β_ℓ (resp. β'_ℓ) not being identical to $\beta_1 = \beta'_1$. Moreover, we get $\alpha \wedge \beta_1 = (-1)^r \omega$ for some r . It follows that

$$\begin{aligned} \langle \alpha \wedge (\beta - \beta'), \omega \rangle_k &= \langle \alpha \wedge \beta, \omega \rangle_k - \langle \alpha \wedge \beta', \omega \rangle_k = \sum a_i \langle \alpha \wedge \beta_i, \omega \rangle_k - \sum b_i \langle \alpha \wedge \beta'_i, \omega \rangle_k \\ &= a_1 \langle \alpha \wedge \beta_1, \omega \rangle_k - b_1 \langle \alpha \wedge \beta'_1, \omega \rangle_k = (a_1 - b_1) \langle \alpha \wedge \beta_1, \omega \rangle_k \\ &= (-1)^r (a_1 - b_1) \langle \omega, \omega \rangle_k = (-1)^r (a_1 - b_1) \neq 0 \end{aligned}$$

Which contradicts $\star\beta = \star\beta'$, so this suffices to show uniqueness.

Now that we have existence and uniqueness, linearity is quite easy. Let $\beta, \gamma \in \Lambda^{k-p}(V)$, then for any α we have

$$\begin{aligned} \langle \alpha, \star(a\beta + b\gamma) \rangle_p &= \langle \alpha \wedge (a\beta + b\gamma), \omega \rangle_k = \langle a\alpha \wedge \beta + b\alpha \wedge \gamma, \omega \rangle_k = a \langle \alpha \wedge \beta, \omega \rangle_k + b \langle \alpha \wedge \gamma, \omega \rangle_k \\ &= a \langle \alpha, \star\beta \rangle_p + b \langle \alpha, \star\gamma \rangle_p = \langle \alpha, a \star\beta + b \star\gamma \rangle \end{aligned}$$

Uniqueness then tells us that $\star(a\beta + b\gamma) = a \star\beta + b \star\gamma$. □

(d) We would like to use (a)-(c) to produce a fiber-wise definition of \star , in such a way that we ensure gluing together these fiberwise maps gives a smooth map on **TODO**

(e) We can use that \star agrees fiberwise with the original fiberwise definition, and in this case identify $dx, dy, dz \leftrightarrow e_1, e_2, e_3$. This in particular means our proof from part (c) shows that if $h \in C^\infty(M, \mathbb{R})$, we get

$$\begin{aligned}\star h dx &= h \star dx = h dy \wedge dz \\ \star h dy &= h \star dy = -h dx \wedge dz \\ \star h dz &= h \star dz = h dx \wedge dy\end{aligned}$$

Now applying this to df , we get

$$\begin{aligned}d \star df &= d \star \left(\frac{\partial}{\partial x} f dx + \frac{\partial}{\partial y} f dy + \frac{\partial}{\partial z} f dz \right) = d \left(\frac{\partial}{\partial x} f dy \wedge dz - \frac{\partial}{\partial y} f dx \wedge dz + \frac{\partial}{\partial z} f dx \wedge dy \right) \\ &= \frac{\partial^2}{\partial x^2} f dx \wedge dy \wedge dz - \frac{\partial^2}{\partial y^2} f dy \wedge dx \wedge dz + \frac{\partial^2}{\partial z^2} f dz \wedge dx \wedge dy \\ &= \left(\frac{\partial^2}{\partial x^2} f + \frac{\partial^2}{\partial y^2} f + \frac{\partial^2}{\partial z^2} f \right) dx \wedge dy \wedge dz\end{aligned}$$

□